changed definition of newfsim, proved horizontal composition

concur/HcompNew.v
@@ -209,21 +209,21 @@ Section FSIM.
   Inductive match_contframes wk wk': frame L1 -> frame L2 -> Prop :=
     match_contframes_intro i s1 s2:
       GS.match_senv cc wk' se1 se2 ->
-      (forall r1 r2 s1', GS.match_reply cc wk r1 r2 ->
+      (forall r1 r2 s1' gw', (get wk) o-> gw' /\ GS.match_reply cc (set wk gw') r1 r2 ->
        Smallstep.after_external (L1 i se1) s1 r1 s1' ->
        exists idx s2',
          Smallstep.after_external (L2 i se2) s2 r2 s2' /\
-         GS.fsim_match_states (HL i) se1 se2 wk' idx s1' s2') ->
-      match_contframes wk wk'
+         exists gw'', gw' *-> gw'' /\ GS.fsim_match_states (HL i) se1 se2 wk' gw'' idx s1' s2') ->
+      match_contframes wk wk' 
         (st L1 i s1)
         (st L2 i s2).
 
-  Inductive match_states: index -> list (frame L1) -> list (frame L2) -> Prop :=
-    | match_states_cons wk idx f1 f2 k1 k2:
-        match_topframes wk idx f1 f2 ->
+  Inductive match_states: GS.gworld cc -> index -> list (frame L1) -> list (frame L2) -> Prop :=
+    | match_states_cons gw wk idx f1 f2 k1 k2:
+        match_topframes wk gw idx f1 f2 ->
         match_cont wk k1 k2 ->
-        match_states idx (f1 :: k1) (f2 :: k2)
-  with match_cont: ccworld cc -> _ -> _ -> Prop :=
+        match_states gw idx (f1 :: k1) (f2 :: k2)
+  with match_cont: GS.ccworld cc -> _ -> _ -> Prop :=
     | match_cont_cons wk wk' f1 f2 k1 k2:
         match_contframes wk wk' f1 f2 ->
         match_cont wk' k1 k2 ->
@@ -232,101 +232,109 @@ Section FSIM.
         match_cont w nil nil.
 
   Inductive order: index -> index -> Prop :=
-    order_intro i x y: fsim_order (HL i) x y -> order (existT _ i x) (existT _ i y).
+    order_intro i x y: GS.fsim_order (HL i) x y -> order (existT _ i x) (existT _ i y).
 
   (** ** Simulation properties *)
 
   Lemma step_simulation:
-    forall idx s1 s2 t s1', match_states idx s1 s2 -> step L1 se1 s1 t s1' ->
+    forall gw idx s1 s2 t s1', match_states gw idx s1 s2 -> step L1 se1 s1 t s1' ->
     exists idx' s2',
       (plus (fun _ => step L2 se2) tt s2 t s2' \/
        star (fun _ => step L2 se2) tt s2 t s2' /\ order idx' idx) /\
-      match_states idx' s1' s2'.
+      exists gw', gw*-> gw' /\ match_states gw' idx' s1' s2'.
   Proof.
-    intros idx s1 s2 t s1' Hs Hs1'.
+    intros gw idx s1 s2 t s1' Hs Hs1'.
     destruct Hs1'; inv Hs.
     - (* internal step *)
-      inv H3; subst_dep. clear idx0.
-      edestruct @fsim_simulation as (idx' & s2' & Hs2' & Hs'); eauto using fsim_lts.
+      inv H4; subst_dep. clear idx0.
+      edestruct @GS.fsim_simulation as (idx' & s2' & Hs2' & Hs'); eauto using GS.fsim_lts.
       eexists (existT _ i idx'), _. split.
       * destruct Hs2'; [left | right]; intuition eauto using star_internal, plus_internal.
         constructor. auto.
-      * econstructor; eauto. econstructor; eauto.
+      * destruct Hs' as [gw' [ACC Hs']].
+        exists gw'. split. auto. econstructor; eauto.
+        econstructor; eauto. 
     - (* cross-component call *)
-      inv H5; subst_dep. clear idx0.
-      edestruct @fsim_match_external as (wx & qx2 & Hqx2 & Hqx & Hsex & Hrx); eauto using fsim_lts.
-      pose proof (fsim_lts (HL j) _ _ Hsex (Hse1 j)).
-      edestruct @fsim_match_initial_states as (idx' & s2' & Hs2' & Hs'); eauto.
+      inv H6; subst_dep. clear idx0.
+      edestruct @GS.fsim_match_external as (wx & qx2 & Hqx2 & ACC & Hqx & Hsex & Hrx); eauto using GS.fsim_lts.
+      pose proof (GS.fsim_lts (HL j) _ _ Hsex (Hse1 j)).
+      edestruct @GS.fsim_match_initial_states as (idx' & s2' & Hs2' & Hs'); eauto.
       eexists (existT _ j idx'), _. split.
       + left. apply plus_one. eapply step_push; eauto 1.
-        erewrite fsim_match_valid_query; eauto.
-      + repeat (econstructor; eauto).
+        erewrite GS.fsim_match_valid_query; eauto.
+      + exists (get wx). split. auto.
+        econstructor.
+        -- econstructor; eauto.
+        -- econstructor; eauto.
+           econstructor; eauto.
+           intros r1 r2 s1' gw'' [ACC1 MR] AF.
+           exploit Hrx; eauto.
     - (* cross-component return *)
-      inv H4; subst_dep. clear idx0.
-      pose proof (fsim_lts (HL i) _ _ H3 H7).
-      edestruct @fsim_match_final_states as (r2 & Hr2 & Hr); eauto.
-      inv H6. inv H8; subst_dep. edestruct H10 as (idx' & s2' & Hs2'& Hs'); eauto.
+      inv H5; subst_dep. clear idx0.
+      pose proof (GS.fsim_lts (HL i) _ _ H3 H8).
+      edestruct @GS.fsim_match_final_states as (r2 & Hr2 & ACC & Hr); eauto.
+      inv H7. inv H6; subst_dep. edestruct H9 as (idx' & s2' & Hs2'& gw'' & ACC2 & Hs'); eauto.
       eexists (existT _ j idx'), _. split.
       + left. apply plus_one. eapply step_pop; eauto.
       + repeat (econstructor; eauto).
   Qed.
 
   Lemma initial_states_simulation:
-    forall q1 q2 s1, match_query cc w q1 q2 -> initial_state L1 se1 q1 s1 ->
-    exists idx s2, initial_state L2 se2 q2 s2 /\ match_states idx s1 s2.
+    forall q1 q2 s1, GS.match_query cc w q1 q2 -> initial_state L1 se1 q1 s1 ->
+    exists idx s2, initial_state L2 se2 q2 s2 /\ match_states (get w) idx s1 s2.
   Proof.
     intros q1 q2 _ Hq [i s1 Hq1 Hs1].
-    pose proof (fsim_lts (HL i) _ _ Hse (Hse1 i)).
-    edestruct @fsim_match_initial_states as (idx & s2 & Hs2 & Hs); eauto.
+    pose proof (GS.fsim_lts (HL i) _ _ Hse (Hse1 i)).
+    edestruct @GS.fsim_match_initial_states as (idx & s2 & Hs2 & Hs); eauto.
     exists (existT _ i idx), (st L2 i s2 :: nil).
     split; econstructor; eauto.
-    + erewrite fsim_match_valid_query; eauto.
+    + erewrite GS.fsim_match_valid_query; eauto.
     + econstructor; eauto.
     + constructor.
   Qed.
 
   Lemma final_states_simulation:
-    forall idx s1 s2 r1, match_states idx s1 s2 -> final_state L1 se1 s1 r1 ->
-    exists r2, final_state L2 se2 s2 r2 /\ match_reply cc w r1 r2.
+    forall wp idx s1 s2 r1, match_states wp idx s1 s2 -> final_state L1 se1 s1 r1 ->
+    exists r2, final_state L2 se2 s2 r2 /\ (get w) o-> wp /\ GS.match_reply cc (set w wp) r1 r2.
   Proof.
-    clear. intros idx s1 s2 r1 Hs Hr1. destruct Hr1 as [i s1 r1 Hr1].
-    inv Hs. inv H4. inv H2. subst_dep. clear idx0.
-    pose proof (fsim_lts (HL i) _ _ H1 H4).
-    edestruct @fsim_match_final_states as (r2 & Hr2 & Hr); eauto.
+    clear. intros wp idx s1 s2 r1 Hs Hr1. destruct Hr1 as [i s1 r1 Hr1].
+    inv Hs. inv H5. inv H3. subst_dep. clear idx0.
+    pose proof (GS.fsim_lts (HL i) _ _ H1 H5).
+    edestruct @GS.fsim_match_final_states as (r2 & Hr2 & ACC & Hr); eauto.
     exists r2. split; eauto. constructor; eauto.
   Qed.
 
   Lemma external_simulation:
-    forall idx s1 s2 qx1, match_states idx s1 s2 -> at_external L1 se1 s1 qx1 ->
-    exists wx qx2, at_external L2 se2 s2 qx2 /\ match_query cc wx qx1 qx2 /\ match_senv cc wx se1 se2 /\
-    forall rx1 rx2 s1', match_reply cc wx rx1 rx2 -> after_external L1 se1 s1 rx1 s1' ->
-    exists idx' s2', after_external L2 se2 s2 rx2 s2' /\ match_states idx' s1' s2'.
+    forall wp idx s1 s2 qx1, match_states wp idx s1 s2 -> at_external L1 se1 s1 qx1 ->
+    exists wx qx2, at_external L2 se2 s2 qx2 /\ wp *-> (get wx) /\ GS.match_query cc wx qx1 qx2 /\ GS.match_senv cc wx se1 se2 /\
+    forall rx1 rx2 s1' wp'', (get wx) o-> wp'' -> GS.match_reply cc (set wx wp'') rx1 rx2 -> after_external L1 se1 s1 rx1 s1' ->
+    exists idx' s2', after_external L2 se2 s2 rx2 s2' /\ exists wp''', wp'' *-> wp''' /\ match_states wp''' idx' s1' s2'.
   Proof.
     clear - HL Hse1.
-    intros idx s1 s2 q1 Hs Hq1. destruct Hq1 as [i s1 qx1 k1 Hqx1 Hvld].
-    inv Hs. inv H2. subst_dep. clear idx0.
-    pose proof (fsim_lts (HL i) _ _ H1 H5) as Hi.
-    edestruct @fsim_match_external as (wx & qx2 & Hqx2 & Hqx & Hsex & H); eauto.
+    intros wp idx s1 s2 q1 Hs Hq1. destruct Hq1 as [i s1 qx1 k1 Hqx1 Hvld].
+    inv Hs. inv H3. subst_dep. clear idx0.
+    pose proof (GS.fsim_lts (HL i) _ _ H1 H6) as Hi.
+    edestruct @GS.fsim_match_external as (wx & qx2 & Hqx2 & ACC & Hqx & Hsex & H); eauto.
     exists wx, qx2. intuition idtac.
     + constructor. eauto.
-      intros j. pose proof (fsim_lts (HL j) _ _ Hsex (Hse1 j)).
-      erewrite fsim_match_valid_query; eauto.
-    + inv H2; subst_dep.
-      edestruct H as (idx' & s2' & Hs2' & Hs'); eauto.
+      intros j. pose proof (GS.fsim_lts (HL j) _ _ Hsex (Hse1 j)).
+      erewrite GS.fsim_match_valid_query; eauto.
+    + inv H3; subst_dep.
+      edestruct H as (idx' & s2' & Hs2' & gw''' & ACC1 & Hs); eauto.
       eexists (existT _ i idx'), _.
       split; repeat (econstructor; eauto).
   Qed.
 
   Lemma semantics_simulation sk1 sk2:
-    GS.fsim_properties cc cc se1 se2 w
+    GS.fsim_properties cc  se1 se2 w
       (semantics L1 sk1 se1)
       (semantics L2 sk2 se2)
       index order match_states.
   Proof.
     split; cbn.
     - intros. unfold valid_query. f_equal.
-      + eapply (fsim_lts (HL true)); eauto.
-      + eapply (fsim_lts (HL false)); eauto.
+      + eapply (GS.fsim_lts (HL true)); eauto.
+      + eapply (GS.fsim_lts (HL false)); eauto.
     - eauto using initial_states_simulation.
     - eauto using final_states_simulation.
     - eauto using external_simulation.
@@ -342,27 +350,27 @@ Definition compose {li} (La Lb: Smallstep.semantics li li) :=
   let L i := match i with true => La | false => Lb end in
   option_map (semantics L) (link (skel La) (skel Lb)).
 
-Lemma compose_simulation {li1 li2} (cc: callconv li1 li2) L1a L1b L1 L2a L2b L2:
-  forward_simulation cc cc L1a L2a ->
-  forward_simulation cc cc L1b L2b ->
+Lemma compose_simulation {li1 li2} (cc: GS.callconv li1 li2) L1a L1b L1 L2a L2b L2:
+  GS.forward_simulation cc L1a L2a ->
+  GS.forward_simulation cc L1b L2b ->
   compose L1a L1b = Some L1 ->
   compose L2a L2b = Some L2 ->
-  forward_simulation cc cc L1 L2.
+  GS.forward_simulation cc L1 L2.
 Proof.
   intros [Ha] [Hb] H1 H2. unfold compose in *. unfold option_map in *.
   destruct (link (skel L1a) (skel L1b)) as [sk1|] eqn:Hsk1; try discriminate. inv H1.
   destruct (link (skel L2a) (skel L2b)) as [sk2|] eqn:Hsk2; try discriminate. inv H2.
   set (L1 := fun i:bool => if i then L1a else L1b).
   set (L2 := fun i:bool => if i then L2a else L2b).
-  assert (HL: forall i, fsim_components cc cc (L1 i) (L2 i)) by (intros [|]; auto).
+  assert (HL: forall i, GS.fsim_components cc (L1 i) (L2 i)) by (intros [|]; auto).
   constructor.
-  eapply Forward_simulation with (order cc L1 L2 HL) (match_states cc L1 L2 HL).
+  eapply GS.Forward_simulation with (order cc L1 L2 HL) (match_states cc L1 L2 HL).
   - destruct Ha, Hb. cbn. congruence.
   - intros se1 se2 w Hse Hse1.
     eapply semantics_simulation; eauto.
     pose proof (link_linkorder _ _ _ Hsk1) as [Hsk1a Hsk1b].
     intros [|]; cbn; eapply Genv.valid_for_linkorder; eauto.
   - clear - HL. intros [i x].
-    induction (fsim_order_wf (HL i) x) as [x Hx IHx].
+    induction (GS.fsim_order_wf (HL i) x) as [x Hx IHx].
     constructor. intros z Hxz. inv Hxz; subst_dep. eauto.
 Qed.
